Some progress on store rule.

mc_reify/set_load_store.v
@@ -4,7 +4,6 @@ Require Import Coq.Logic.JMeq.
 Local Open Scope logic.
 
 Require Export mc_reify.reify.
-Require Export mc_reify.bool_funcs.
 Require Import mc_reify.set_reif.
 Require Import MirrorCore.Lemma.
 Require Import MirrorCharge.RTac.ReifyLemma.
@@ -171,24 +170,24 @@ Defined.
 
 Lemma semax_store_localD:
     forall (temp : PTree.t (type * bool)) (var : PTree.t type) 
-     (ret : type) (gt : PTree.t type) (id : ident) (t t_root : type) (e0 e1 e2: Clight.expr)
+     (ret : type) (gt : PTree.t type) (t t_root : type) (e0 e1 e2: Clight.expr)
      (efs : list efield) (tts : list type) 
      (e : type_id_env) (lr : LLRR) (n: nat)
      sh P T1 T2 R gs Post
       (gfs: list gfield)
-      (p p': val) (v0: val) (v': reptype t_root) lr,
+      (p p': val) (v0: val) (v': reptype t_root),
   forall {Espec: OracleKind},
       typeof (nested_efield e1 efs tts) = t ->
       type_is_by_value t = true ->
-      legal_nested_efield e t_root e1 gfs tts lr = true ->
-      msubst_eval_LR T1 T2 e1 lr = Some p ->
-      msubst_eval_LR T1 T2 (Ecast e2 t) RRRR = Some v0 ->
-      msubst_efield_denote T1 T2 efs = Some gfs ->
       tc_LR_b_norho (mk_tycontext temp var ret gt gs) e1 lr = true ->
       tc_LR_b_norho (mk_tycontext temp var ret gt gs) (Ecast e2 (typeof (nested_efield e1 efs tts))) RRRR = true ->
       tc_efield_b_norho (mk_tycontext temp var ret gt gs) efs = true ->
+      msubst_efield_denote T1 T2 efs = Some gfs ->
+      msubst_eval_LR T1 T2 e1 lr = Some p ->
+      msubst_eval_LR T1 T2 (Ecast e2 t) RRRR = Some v0 ->
+      legal_nested_efield e t_root e1 gfs tts lr = true ->
 
-      writable_share_b sh = true ->
+      writable_share sh ->
       (@eq (option mpred)) (nth_error R n) (Some (data_at sh t_root v' p')) ->
   (forall rho, 
       !!(tc_environ (mk_tycontext temp var ret gt gs) rho) && (assertD P (localD T1 T2) R rho) |-- !! (p = p')) ->
@@ -218,7 +217,6 @@ Proof.
     f_equal.
   } Unfocus.
   subst Post e0.
-  apply writable_share_b_sound in H8.
   eapply semax_extract_later_prop'.
   Focus 1. {
     rewrite <- insert_local.
@@ -236,21 +234,20 @@ Proof.
       unfold assertD; entailer!.
     - intro rho.
       apply prop_right.
-      eapply tc_expr_b_sound.
-      exact H6.
+      eapply tc_expr_b_sound; auto.
     - intro rho.
       unfold local, lift1; simpl; apply prop_right.
       apply tc_efield_b_sound; auto.
 Qed.
 
 Definition store_lemma (temp : PTree.t (type * bool)) (var : PTree.t type) 
-     (ret : type) (gt : PTree.t type) (id : ident) (t t_root : type) (e0 e1 e2: Clight.expr)
+     (ret : type) (gt : PTree.t type) (t t_root : type) (e0 e1 e2: Clight.expr)
      (efs : list efield) (tts : list type) 
      (e : type_id_env) (lr : LLRR) (n: nat): my_lemma.
-reify_lemma reify_vst (semax_store_localD temp var ret gt id t t_root e0 e1 e2 efs tts e lr n).
+reify_lemma reify_vst (semax_store_localD temp var ret gt t t_root e0 e1 e2 efs tts e lr n).
 Defined.
 
-Print store_lemma.
+(* Print store_lemma. *)
 
 Section tbled.
 Variable n : nat.
@@ -273,21 +270,8 @@ Existing Instance MA.
 
 Existing Instance rtac_base.MentionsAnyOk.
 
-Lemma APPLY_sound_load_lemma: forall (temp : PTree.t (type * bool)) (var : PTree.t type) 
-  (ret : type) (gt : PTree.t type) (id : ident) (t t_root : type)
-  (e0 e1 : Clight.expr) (efs : list efield) (tts : list type)
-  (e : type_id_env) (lr : LLRR) (n : nat), 
-  rtac_sound (EAPPLY typ func (load_lemma temp var ret gt id t t_root e0 e1 efs tts e lr n)).
-Proof.
-  intros.
-  apply EAPPLY_sound; auto with typeclass_instances.
-  + apply APPLY_condition1.
-  + apply APPLY_condition2.
-  + unfold Lemma.lemmaD, split_env, Lemma.lemmaD'. simpl.
-(* Set Printing Depth 200. *)
-    unfold exprD'_typ0. simpl.
-    unfold exprD'. simpl.
-    assert (@funcAs typ func RType_typ
+Lemma load_store_sound_aux:
+  forall t_root, (@funcAs typ func RType_typ
               (func_defs.RSym_sym tbl)
               (@inr
                  (sum
@@ -303,15 +287,71 @@ Proof.
             Some
               (fun (sh : share) (rt : typD (reptyp t_root)) (v : val) =>
                data_at sh t_root (reptyp_reptype t_root rt) v)).
+Proof.
+  intros.
+  unfold funcAs; simpl.
+  assert (forall pl: (fun t0 : typ =>
+    {tyArr t0 (tyArr (reptyp t_root) (tyArr tyval tympred)) =
+     tyArr tyshare (tyArr (reptyp t_root) (tyArr tyval tympred))} +
+    {tyArr t0 (tyArr (reptyp t_root) (tyArr tyval tympred)) <>
+     tyArr tyshare (tyArr (reptyp t_root) (tyArr tyval tympred))})
+     tyshare, pl = left eq_refl).
+  Focus 1. {
+    intros.
+    destruct pl; [f_equal; apply proof_irr | congruence].
+  } Unfocus.
+  match goal with 
+  | [ |- context [match (match ?e with _ => _ end) with _ => _ end] ] => rewrite (H e)
+  end.
+  unfold Rcast; simpl.
+  reflexivity.
+Qed.
+
+Lemma APPLY_sound_store_lemma: forall (temp : PTree.t (type * bool)) (var : PTree.t type) 
+  (ret : type) (gt : PTree.t type) (t t_root : type)
+  (e0 e1 e2 : Clight.expr) (efs : list efield) (tts : list type)
+  (e : type_id_env) (lr : LLRR) (n : nat), 
+  rtac_sound (EAPPLY typ func (store_lemma temp var ret gt t t_root e0 e1 e2 efs tts e lr n)).
+Proof.
+  intros.
+  apply EAPPLY_sound; auto with typeclass_instances.
+  + apply APPLY_condition1.
+  + apply APPLY_condition2.
+  + unfold Lemma.lemmaD, split_env, Lemma.lemmaD'. simpl.
+    unfold exprD'_typ0. simpl.
+    unfold exprD'. simpl.
+
+    rewrite (load_store_sound_aux t_root); simpl.
+    assert (@funcAs typ func RType_typ
+                (func_defs.RSym_sym tbl)
+                (@inr
+                (sum
+                (sum SymEnv.func
+                (ILogicFunc.ilfunc typ))
+                (BILogicFunc.bilfunc typ))
+                func'
+                (Sep (fupd_val t_root)))
+                (tyArr 
+                (tylist tygfield)
+                (tyArr 
+                (reptyp t_root)
+                (tyArr tyval
+                (reptyp t_root))))
+      = Some
+         (fun (gfs : list gfield) (v : typD (reptyp t_root)) (v0 : val) =>
+          reptype_reptyp t_root (upd_val t_root gfs (reptyp_reptype t_root v) v0))).
     Focus 1. {
       intros.
-      unfold funcAs; simpl.
+      unfold funcAs.
+      simpl.
       assert (forall pl: (fun t0 : typ =>
-        {tyArr t0 (tyArr (reptyp t_root) (tyArr tyval tympred)) =
-         tyArr tyshare (tyArr (reptyp t_root) (tyArr tyval tympred))} +
-        {tyArr t0 (tyArr (reptyp t_root) (tyArr tyval tympred)) <>
-         tyArr tyshare (tyArr (reptyp t_root) (tyArr tyval tympred))})
-         tyshare, pl = left eq_refl).
+        {tyArr t0 (tyArr (reptyp t_root) (tyArr tyval (reptyp t_root))) =
+         tyArr (tylist tygfield)
+           (tyArr (reptyp t_root) (tyArr tyval (reptyp t_root)))} +
+        {tyArr t0 (tyArr (reptyp t_root) (tyArr tyval (reptyp t_root))) <>
+         tyArr (tylist tygfield)
+           (tyArr (reptyp t_root) (tyArr tyval (reptyp t_root)))})
+         (tylist tygfield), pl = left eq_refl).
       Focus 1. {
         intros.
         destruct pl; [f_equal; apply proof_irr | congruence].
@@ -323,6 +363,29 @@ Proof.
       reflexivity.
     } Unfocus.
     rewrite H. simpl. clear H.
+    intros.
+    unfold exprT_App, exprT_Inj, Rcast_val, Rcast in *. simpl in *.
+    unfold ModularFunc.ILogicFunc.typ2_cast_quant, ModularFunc.ILogicFunc.typ2_cast_bin in *; simpl in *.
+    eapply semax_store_localD; eauto.
+    rewrite reptyp_reptype_reptype_reptyp in H12.
+    exact H12.
+Qed.
+
+Lemma APPLY_sound_load_lemma: forall (temp : PTree.t (type * bool)) (var : PTree.t type) 
+  (ret : type) (gt : PTree.t type) (id : ident) (t t_root : type)
+  (e0 e1 : Clight.expr) (efs : list efield) (tts : list type)
+  (e : type_id_env) (lr : LLRR) (n : nat), 
+  rtac_sound (EAPPLY typ func (load_lemma temp var ret gt id t t_root e0 e1 efs tts e lr n)).
+Proof.
+  intros.
+  apply EAPPLY_sound; auto with typeclass_instances.
+  + apply APPLY_condition1.
+  + apply APPLY_condition2.
+  + unfold Lemma.lemmaD, split_env, Lemma.lemmaD'. simpl.
+(* Set Printing Depth 200. *)
+    unfold exprD'_typ0. simpl.
+    unfold exprD'. simpl.
+    rewrite (load_store_sound_aux t_root); simpl.
     assert (exprT_GetVAs []
                   [tyOracleKind; 
                 reptyp t_root; tyval; tyval; tyval;
