mc_reify/funcs.v
@@ -202,7 +202,6 @@ match v with
 | fVsingle => Vsingle
 | fVundef => Vundef
 end.
-Locate binary_operation.
 
 Inductive eval :=
 | feval_cast : type -> type -> eval
@@ -339,8 +338,6 @@ Inductive sep :=
 | fupd_val : type -> sep
 (*| flseg : forall (t: type) (i : ident), listspec t i -> sep*)
 . 
-
-Locate is_Fnil.
 
 Fixpoint reptyp (ty: type) : typ :=
   match ty with
@@ -507,8 +504,35 @@ match
         end
    end.
 
+Lemma reptyp_reptype_reptype_reptyp: forall t v, reptyp_reptype t (reptype_reptyp t v) = v.
+Proof.
+  intros.
+  eapply (type_mut
+    (fun t => forall v, reptyp_reptype t (reptype_reptyp t v) = v)
+    (fun tl => True)
+    (fun fld => (forall v, reptyp_structlist_reptype fld (reptype_structlist_reptyp fld v) = v) /\
+                (forall v, reptyp_unionlist_reptype fld (reptype_unionlist_reptyp fld v) = v)));
+  intros; simpl; auto.
+  + rewrite map_map.
+    induction v0; simpl; auto.
+    rewrite H, IHv0.
+    reflexivity.
+  + apply (proj1 H).
+  + apply (proj2 H).
+  + split.
+    - if_tac; [apply H |].
+      intros.
+      unfold fst, snd.
+      rewrite H, (proj1 H0).
+      destruct v0; reflexivity.
+    - if_tac; [apply H |].
+      intros.
+      destruct v0; [rewrite H; auto |].
+      rewrite (proj2 H0).
+      reflexivity.
+Qed.
+
 Definition sepD  (s : sep) : typD  (typeof_sep s).
-Check data_at.
 refine
 match s with
 | flocal => (local : typD (typeof_sep flocal))
@@ -569,7 +593,9 @@ Inductive smx :=
 | fstruct_field
 | funion_field
 | farray_subsc
-| fwritable_share_b
+| fwritable_share
+| fTsh
+| fEws
 | ftype_is_by_value
 .
 
@@ -622,7 +648,9 @@ match t with
 | fstruct_field => tyArr tyident tygfield
 | funion_field => tyArr tyident tygfield
 | farray_subsc => tyArr tyZ tygfield
-| fwritable_share_b => tyArr tyshare tybool
+| fwritable_share => tyArr tyshare typrop
+| fTsh => tyshare
+| fEws => tyshare
 | ftype_is_by_value => tyArr tyc_type tybool
 end.
 
@@ -662,7 +690,9 @@ match t with
 | fstruct_field => StructField
 | funion_field => UnionField
 | farray_subsc => ArraySubsc
-| fwritable_share_b => writable_share_b
+| fwritable_share => writable_share
+| fTsh => SeparationLogic.Tsh
+| fEws => assert_lemmas.Ews
 | ftype_is_by_value => client_lemmas.type_is_by_value
 end.
 
