mc_reify/verif_sha_bdo7.v
@@ -558,8 +558,9 @@ canonicalize.
 *)
 (* Set Printing Depth 4. *)
 Time run_rtac reify_vst term_table (SYMEXE_sound 20). (* 3.9 seconds *)
-repeat (split; try eexists).
-Print _s1.
+repeat (split; repeat eexists).
+Print _X.
+Print _T1.
 admit.
 Time Qed.
 repeat split.
